progress

src/LibListSorted.v
@@ -10,31 +10,32 @@ Require Import LibTactics LibLogic LibRelation LibWf LibList
 
 
 (* ********************************************************************** *)
-(** * Permutations of lists *)
-
-Section Permutation.
-Variable A : Type.
+(** * List permutation *)
 
 (* ---------------------------------------------------------------------- *)
 (** ** Definition *)
 
-(** We could define permutation in terms of multisets,
-    but this would impose additional constraints on the
-    type of elements. So instead, we use a definition
-    in terms of permutation of two inner segment of lists,
-    taking the reflexive-transitive closure. *)
+(** We consider a particular definition of [permut], but there would
+    be many other equivalent definitions. Users of this library should 
+    not manipulate the definition directly, but instead work exclusively
+    using the properties of [permut], established in this file. *)
 
-Inductive permut_one : list A -> list A -> Prop :=
+Inductive permut_one (A:Type) : list A -> list A -> Prop :=
   | permut_one_intro : forall l1 l2 l3 l4,
       permut_one (l1++l2++l3++l4) (l1++l3++l2++l4).
 
-Hint Constructors permut_one.
-
-Definition permut := rtclosure permut_one.
+Definition permut (A:Type) := rtclosure (@permut_one A).
 
 
 (* ---------------------------------------------------------------------- *)
 (** ** Properties *)
+
+Section PermutProp.
+Variables (A : Type).
+Implicit Types l : list A.
+Implicit Types P : A->Prop.
+
+Hint Constructors permut_one.
 
 (** Permutation is an equivalence *)
 
@@ -43,35 +44,35 @@ Lemma permut_refl : forall l,
 Proof using. intros. apply rtclosure_refl. Qed.
 
 Lemma permut_sym : forall l1 l2,
-  permut l1 l2 -> permut l2 l1.
+  permut l1 l2 -> 
+  permut l2 l1.
 Proof using.
   intros. induction H.
-  apply permut_refl.
-  applys rtclosure_last. apply IHrtclosure. inverts~ H.
+  { apply permut_refl. }
+  { applys rtclosure_last. apply IHrtclosure. inverts~ H. }
 Qed.
+
+Lemma permut_sym_eq : forall l1 l2,
+  permut l1 l2 = permut l2 l1.
+Proof using. intros. hint permut_sym. extens*. Qed.
 
 Lemma permut_trans : forall l2 l1 l3,
-  permut l1 l2 -> permut l2 l3 -> permut l1 l3.
+  permut l1 l2 -> 
+  permut l2 l3 -> 
+  permut l1 l3.
 Proof using. intros. apply* rtclosure_trans. Qed.
 
-(** Permutation is a congruence with respect to [++] and [::] *)
-
-Lemma permut_flip : forall l1 l2,
-  permut (l1++l2) (l2++l1).
-Proof using.
-  intros. lets: (permut_one_intro nil l1 l2 nil).
-  rew_app in *. apply~ rtclosure_once.
-Qed.
+(** Permutation is a congruence with respect to [++] *)
 
 Lemma permut_app_l : forall l1 l1' l2,
   permut l1 l1' ->
   permut (l1 ++ l2) (l1' ++ l2).
 Proof using.
   introv H. gen l2. induction H; intros.
-  apply permut_refl.
-  specializes IHrtclosure l2. inverts H.
-   rew_app in *. eapply permut_trans.
-   applys* rtclosure_step. apply permut_refl.
+  { apply permut_refl. }
+  { specializes IHrtclosure l2. inverts H.
+    rew_list in *. applys permut_trans.
+    { applys* rtclosure_step. } { apply permut_refl. } }
 Qed.
 
 Lemma permut_app_r : forall l1 l2 l2',
@@ -79,67 +80,101 @@ Lemma permut_app_r : forall l1 l2 l2',
   permut (l1 ++ l2) (l1 ++ l2').
 Proof using.
   introv H. gen l1. induction H; intros.
-  apply permut_refl.
-  specializes IHrtclosure l1. inverts H.
-   rewrite <- app_assoc in *. eapply permut_trans.
-   applys* rtclosure_step. apply permut_refl.
+  { apply permut_refl. }
+  { specializes IHrtclosure l1. inverts H.
+    rewrite <- app_assoc in *. applys permut_trans.
+    { applys* rtclosure_step. } { apply permut_refl. } }
 Qed.
 
 Lemma permut_app_lr : forall l1 l1' l2 l2',
-  permut l1 l1' -> permut l2 l2' ->
+  permut l1 l1' -> 
+  permut l2 l2' ->
   permut (l1 ++ l2) (l1' ++ l2').
 Proof using.
   intros. applys rtclosure_trans.
-  sapply* permut_app_l.
-  apply* permut_app_r.
+  { applys* permut_app_l. } { apply* permut_app_r. }
 Qed.
 
-Lemma permut_cons : forall x l1 l1',
-  permut l1 l1' ->
-  permut (x::l1) (x::l1').
+Lemma permut_cons : forall x l1 l2,
+  permut l1 l2 ->
+  permut (x::l1) (x::l2).
 Proof using.
-  intros. lets: (@permut_app_r (x::nil) _ _ H).
-  rew_app in *. auto.
+  intros. lets: (@permut_app_r (x::nil) _ _ H). rew_list~ in *.
 Qed.
 
-(** Permutation are stable through list reversal *)
+Lemma permut_last : forall x l1 l2,
+  permut l1 l2 ->
+  permut (l1&x) (l2&x).
+Proof using.
+  intros. applys~ permut_app_lr. applys permut_refl.
+Qed.
+
+(** Other results *)
+
+Lemma mem_permut_inv_r : forall l1 l2 x,
+  mem x l1 ->
+  permut l1 l2 ->
+  mem x l2.
+Proof using.
+  introv M K. gen M. induction K as [|l2 l1 l3 H]; intros.
+  { auto. }
+  { inverts H. applys (rm IHK). repeat rewrite mem_app_eq in *. autos*. }
+Qed.
+
+Lemma mem_permut_inv_l : forall l1 l2 x,
+  mem x l1 ->
+  permut l2 l1 ->
+  mem x l2.
+Proof using.
+  introv M K. hint permut_sym, mem_permut_inv_r. autos*. 
+Qed. 
+
+Lemma permut_flip : forall l1 l2,
+  permut (l1 ++ l2) (l2 ++ l1).
+Proof using.
+  intros. lets: (permut_one_intro nil l1 l2 nil).
+  rew_list in *. apply~ rtclosure_once.
+Qed.
 
 Lemma permut_rev : forall l,
   permut l (rev l).
 Proof using.
-  induction l. apply permut_refl. rew_rev.
-  lets: (@permut_flip (a::nil) (rev l)). rew_app in *.
-  apply~ (@permut_trans (a::rev l)). apply~ permut_cons.
+  intros. induction l. apply permut_refl. rew_list.
+  lets M: (@permut_flip (a::nil) (rev l)). rew_list in M.
+  applys~ permut_trans M. apply~ permut_cons.
 Qed.
 
-(** Properties of elements are preserved by permutation *)
-
-Lemma Forall_permut_one : forall (P:A->Prop) l1 l2,
-  Forall P l1 -> permut_one l1 l2 -> Forall P l2.
+Lemma Forall_permut_inv : forall P l1 l2,
+  Forall P l1 -> 
+  permut l1 l2 -> 
+  Forall P l2.
 Proof using.
-  introv F Per. inverts Per.
-  lets F0 F345: (Forall_app_inv _ _ F).
-  lets F3 F45: (Forall_app_inv _ _ F345).
-  lets F4 F5: (Forall_app_inv _ _ F45).
-  apply~ Forall_app. apply~ Forall_app. apply~ Forall_app.
-Qed.
+  introv F K. rewrite Forall_iff_forall_mem in *.
+  introv M. applys F. applys* mem_permut_inv_l M K.
+Qed.  (* COQBUG? why [applys* mem_permut_inv_l] does not work *)
 
-Lemma Forall_permut : forall (P:A->Prop) l1 l2,
-  Forall P l1 -> permut l1 l2 -> Forall P l2.
+Lemma Exists_permut_inv : forall P l1 l2,
+  Exists P l1 -> 
+  permut l1 l2 -> 
+  Exists P l2.
 Proof using.
-  introv F1 Per. gen F1. induction Per.
-  auto.
-  autos* Forall_permut_one.
-Qed.
+  introv. do 2 rewrite Exists_iff_exists_mem. intros (x&M&Px) K.
+  hint mem_permut_inv_r. autos*.
+Qed.  (* COQBUG? why [applys* mem_permut_inv_l] does not work *)
 
-End Permutation.
+End PermutProp.
 
-Hint Resolve permut_refl permut_flip
-             permut_app_lr permut_cons.
+Hint Resolve permut_refl permut_flip permut_app_lr permut_cons
+  permut_last permut_rev.
 
 
 (* ---------------------------------------------------------------------- *)
 (** ** Permutation tactic *)
+
+(** [permut_simpl] simplifies a goal of the form
+    [permut l l'] where [l] and [l'] are lists built with
+    concatenation and consing, by cancelling syntactically
+    equal elements. *)
 
 Section PermutationTactic.
 Variable A : Type.
@@ -148,18 +183,21 @@ Implicit Types l : list A.
 Lemma permut_get_1 : forall l1 l2,
   permut (l1 ++ l2) (l1 ++ l2).
 Proof using. intros. apply permut_refl. Qed.
+
 Lemma permut_get_2 : forall l1 l2 l3,
   permut (l1 ++ l2 ++ l3) (l2 ++ l1 ++ l3).
 Proof using.
   intros. apply rtclosure_once.
   applys (@permut_one_intro _ nil l1 l2 l3).
 Qed.
+
 Lemma permut_get_3 : forall l1 l2 l3 l4,
   permut (l1 ++ l2 ++ l3 ++ l4) (l2 ++ l3 ++ l1 ++ l4).
 Proof using.
   intros. do 2 rewrite <- (@app_assoc _ l2).
   apply permut_get_2.
 Qed.
+
 Lemma permut_get_4 : forall l1 l2 l3 l4 l5,
   permut (l1 ++ l2 ++ l3 ++ l4 ++ l5)
          (l2 ++ l3 ++ l4 ++ l1 ++ l5).
@@ -167,6 +205,7 @@ Proof using.
   intros. do 2 rewrite <- (@app_assoc _ l2).
   apply permut_get_3.
 Qed.
+
 Lemma permut_get_5 : forall l1 l2 l3 l4 l5 l6,
   permut (l1 ++ l2 ++ l3 ++ l4 ++ l5 ++ l6)
          (l2 ++ l3 ++ l4 ++ l5 ++ l1 ++ l6).
@@ -174,6 +213,7 @@ Proof using.
   intros. do 2 rewrite <- (@app_assoc _ l2).
   apply permut_get_4.
 Qed.
+
 Lemma permut_get_6 : forall l1 l2 l3 l4 l5 l6 l7,
   permut (l1 ++ l2 ++ l3 ++ l4 ++ l5 ++ l6 ++ l7)
          (l2 ++ l3 ++ l4 ++ l5 ++ l6 ++ l1 ++ l7).
@@ -205,7 +245,6 @@ Proof using. introv P1 P2. apply~ (permut_trans P2 P1). Qed.
 
 End PermutationTactic.
 
-
 (** [permut_prepare] applies to a goal of the form [permut l l']
     and sets [l] and [l'] in the form [l1 ++ l2 ++ .. ++ nil],
     (some of the lists [li] are put in the form [x::nil]). *)
@@ -227,7 +266,7 @@ Ltac permut_isolate_cons :=
     match goal with |- context [?x::?l] =>
       match l with
       | nil => fail 1
-      | _ => rewrite <- (@app_cons_one _ x l)
+      | _ => rewrite <- (@app_cons_one_r _ x l)
       end
     end.
 
@@ -237,12 +276,6 @@ Ltac permut_simpl_prepare :=
    autorewrite with permut_rew;
    apply permut_tactic_setup;
    repeat rewrite app_assoc.
-
-
-(** [permut_simplify] simplifies a goal of the form
-    [permut l l'] where [l] and [l'] are lists built with
-    concatenation and consing, by cancelling syntactically
-    equal elements *)
 
 Ltac permut_index_of l lcontainer :=
   match constr:(lcontainer) with
@@ -274,245 +307,158 @@ Ltac permut_simpl :=
   autorewrite with permut_rew;
   try apply permut_refl.
 
-(* todo: permut rewrite *)
 
 
 (* ********************************************************************** *)
 (** * Sorted lists *)
 
 (* ---------------------------------------------------------------------- *)
-(** ** Definition *)
+(** ** [heads_le] *)
 
-Section Sorted.
-Variable A : Type.
-Implicit Types le : binary A.
+(** [head_le x l] asserts that the head of [l], if any, is smaller 
+    than [x] w.r.t. [le]. It will be useful to state lemmas about [sorted]. *)
 
-Inductive sorted le : list A -> Prop :=
-  | sorted_nil : sorted le nil
-  | sorted_one : forall x, sorted le (x::nil)
-  | sorted_two : forall x y l,
-     sorted le (y::l) -> le x y ->
-     sorted le (x::y::l).
-
-Definition rsorted le := sorted (flip le).
-
-Definition head_of_le le x l :=
+Definition head_le A (le : binary A) x l :=
   match l with
   | nil => True
   | h::_ => le x h
   end.
 
-Definition head_le le l1 l2 :=
-  match l1,l2 with
-  | _,nil => True
-  | nil,_ => True
-  | h1::_,h2::_ => le h1 h2
-  end.
+Section HeadLe.
+Variables (A : Type) (le : binary A).
+Implicit Types l : list A.
+
+Lemma head_le_trans : forall x y l,
+  trans le ->
+  head_le le x l ->
+  le y x ->
+  head_le le y l.
+Proof using.
+  introv Tr H L. destruct l; simpls. { auto. } { applys* Tr. }
+Qed.
+
+Lemma Forall_le_head_le : forall x l,
+  Forall (le x) l -> 
+  head_le le x l.
+Proof using. introv H. destruct l; simpls. auto. inverts~ H. Qed.
+
+End HeadLe.
+
+
+(* ---------------------------------------------------------------------- *)
+(** ** Properties of [sorted] *)
+
+(** [sorted le l] asserts that [l] is sorted w.r.t. [le] *)
+
+Inductive sorted A (le : binary A) : list A -> Prop :=
+  | sorted_nil : 
+      sorted le nil
+  | sorted_one : forall x, 
+      sorted le (x::nil)
+  | sorted_two : forall x y l,
+      sorted le (y::l) -> 
+      le x y ->
+      sorted le (x::y::l).
+
+Section Sorted.
+Variables (A : Type) (le : binary A).
+Hint Constructors sorted.
+
+(** Constructor: if [l] is sorted and [x] is smaller than the head
+   of [l], then [x::l] is sorted. *)
+
+Lemma sorted_cons : forall l x,
+  sorted le l -> 
+  head_le le x l -> 
+  sorted le (x::l).
+Proof using. introv S Hd. inverts~ S. Qed.
+
+(** Inversion *)
+
+Lemma sorted_cons_inv : forall x l,
+  sorted le (x::l) -> 
+  head_le le x l /\ sorted le l.
+Proof using. introv H. inverts H; simpls~. Qed.
+
+Lemma sorted_cons_inv_head_le : forall x l,
+  sorted le (x::l) -> 
+  head_le le x l.
+Proof using. introv H. inverts H; simpls~. Qed.
+
+Lemma sorted_cons_inv_sorted : forall x l,
+  sorted le (x::l) -> 
+  sorted le l.
+Proof using. introv H. inverts~ H. Qed.
+
+(** Key lemma: if [l] is sorted and [x] is smaller than the
+   head of [l], then [x] is smaller than all elements in [l]. *)
+
+Lemma Forall_le_from_sorted_head_le : forall x l,
+  trans le ->
+  sorted le l ->
+  head_le le x l ->
+  Forall (le x) l.
+Proof using.
+  intros x l. induction l; introv Tr S L.
+  { constructor~. }
+  { simpls. lets (N&M): (sorted_cons_inv S). constructor~. apply~ IHl.
+    applys* head_le_trans. }
+Qed.
 
 End Sorted.
 
-(* ---------------------------------------------------------------------- *)
-(** ** Properties about sorted *)
-
-Implicit Arguments sorted [A].
-Hint Unfold rsorted.
-
-Section SortedProperties.
-Hint Constructors sorted.
-
-Variables (A : Type).
-Variable le : binary A.
-Hint Resolve sorted_nil sorted_one.
-
-Lemma sorted_inv : forall x l,
-  sorted le (x::l) -> head_of_le le x l /\ sorted le l.
-Proof using. introv H. inverts H; simpls~. Qed.
-
-Lemma sorted_sub : forall x l,
-  sorted le (x::l) -> sorted le l.
-Proof using. introv H. inverts~ H. Qed.
-
-Lemma sorted_cons : forall l,
-  sorted le l -> forall x,
-  head_of_le le x l -> sorted le (x::l).
-Proof using. introv S Hd. inverts~ S. Qed.
-
-Lemma head_le_from_sorted : forall x l1 l2,
-  sorted le (x::l2) ->
-  head_le le l1 (x::l2) ->
-  head_le le (x::l1) l2.
-Proof using.
-  intros. destruct l2; simpl. auto. inverts~ H.
-Qed.
-
-Lemma sorted_cons_head_of : forall x l,
-  sorted le (x::l) -> head_of_le le x l.
-Proof using. introv H. inverts H; simpls~. Qed.
-
-Lemma head_le_nil_l : forall l,
-  head_le le nil l.
-Proof using. intros. unfolds. destruct~ l. Qed.
-
-Lemma head_le_nil_r : forall l,
-  head_le le l nil.
-Proof using. intros. unfolds. destruct~ l. Qed.
-
-Lemma sorted_cons_head : forall l1 l2 x,
-  head_le le (x::l1) l2 ->
-  sorted le l2 ->
-  sorted le (x::l2).
-Proof using. introv H S2. destruct l2. auto. apply~ sorted_cons. Qed.
-
-Lemma head_le_flip : forall l1 l2,
-  head_le (flip le) l1 l2 = head_le le l2 l1.
-Proof using. destruct l1; destruct l2; auto. Qed.
-
-Lemma head_le_flip_1 : forall l1 l2,
-  head_le (flip le) l1 l2 -> head_le le l2 l1.
-Proof using. intros. rewrite~ <- head_le_flip. Qed.
-
-Lemma head_le_flip_2 : forall l1 l2,
-  head_le le l2 l1 -> head_le (flip le) l1 l2.
-Proof using. intros. rewrite~ head_le_flip. Qed.
-
-Lemma sorted_Forall_le : forall x l,
-  total_preorder le ->
-  head_of_le le x l -> sorted le l -> Forall (le x) l.
-Proof using.
-  induction l; simpl; introv Tot LeH Sl. auto. constructor~.
-  lets: (sorted_sub Sl). constructor~. apply~ IHl.
-  destruct~ l; simpls~. inverts Sl. sapply* total_preorder_trans.
-Qed.
-
-Lemma head_of_le_Forall_le : forall x l,
-  Forall (le x) l -> head_of_le le x l.
-Proof using. introv H. destruct l; simpls. auto. inverts~ H. Qed.
-
-Lemma sorted_flip_flip : forall l,
-  sorted le l ->
-  sorted (flip (flip le)) l.
-Proof using.
-  introv H. rewrite flip_flip. induction H.
-   constructor. constructor. apply~ sorted_cons.
-Qed.
-
-End SortedProperties.
-
-(* ---------------------------------------------------------------------- *)
-(** ** Properties about rsorted *)
-
-Section RSortedProperties.
-Variables (A : Type).
-Variable le : binary A.
-Hint Resolve sorted_nil sorted_one.
-Hint Constructors sorted.
-
-Lemma rsorted_inv : forall x l,
-  rsorted le (x::l) -> head_of_le (flip le) x l /\ rsorted le l.
-Proof using. introv H. inverts H; simpls~. Qed.
-
-Lemma head_le_from_rsorted : forall x l1 l2,
-  rsorted le (x::l2) ->
-  head_le (flip le) l1 (x::l2) ->
-  head_le (flip le) (x::l1) l2.
-Proof using.
-  intros. destruct l2; simpl. auto. inverts~ H.
-Qed.
-
-Lemma rsorted_cons_head : forall l1 l2 x,
-  head_le (flip le) (x::l1) l2 ->
-  rsorted le l2 ->
-  rsorted le (x::l2).
-Proof using. introv H S2. destruct~ l2. Qed.
-
-Lemma sorted_app : forall l1 l2,
-  head_le le l1 l2 -> rsorted le l1 -> sorted le l2 ->
-  sorted le ((rev l1) ++ l2).
-Proof using.
-  introv. gen l2. induction l1; introv Hd S1 S2; rew_rev. auto.
-  lets Hd1 S1': (rsorted_inv S1). clear S1.
-  apply IHl1. destruct~ l1. auto.
-  apply sorted_cons. auto. destruct~ l2.
-Qed.
-
-End RSortedProperties.
-
-Lemma rsorted_app : forall (A : Type) (le : binary A) l1 l2,
-  head_le le l2 l1 -> sorted le l1 -> rsorted le l2 ->
-  rsorted le ((rev l1) ++ l2).
-Proof using.
-  unfold rsorted. intros. apply sorted_app.
-    rewrite~ head_le_flip.
-    unfolds. apply~ sorted_flip_flip.
-    auto.
-Qed.
 
 
 (* ********************************************************************** *)
 (** * Sorting of a list *)
+
+(* ---------------------------------------------------------------------- *)
+(** ** Definition *)
+
+(** [sorts le l l'] asserts that [l'] is the result of sorting
+    [l] w.r.t. [le]. *)
+
+Definition sorts A (le : binary A) (l l' : list A) : Prop :=
+  permut l l' /\ sorted le l'.
+
+
+(* ---------------------------------------------------------------------- *)
+(** ** Properties *)
 
 Section Sorts.
 Variables (A : Type).
 Implicit Types le : binary A.
 Hint Resolve sorted_nil sorted_one.
 
-(* ---------------------------------------------------------------------- *)
-(** ** Definition *)
-
-Definition sorts le l l' :=
-  permut l l' /\ sorted le l'.
-
-Definition rsorts le := sorts (flip le).
-
-
-(* ---------------------------------------------------------------------- *)
-(** ** Properties *)
-
 Lemma sorts_refl : forall le l,
-  sorted le l -> sorts le l l.
+  sorted le l -> 
+  sorts le l l.
 Proof using. split. apply permut_refl. auto. Qed.
 
-Lemma rsorts_refl : forall le l,
-  rsorted le l -> rsorts le l l.
-Proof using. intros. apply~ sorts_refl. Qed.
-
-Lemma sorts_app_rev : forall le l1 l2,
- head_le le l1 l2 -> rsorted le l1 -> sorted le l2 ->
- sorts le (l1 ++ l2) (rev l1 ++ l2).
-Proof using.
-  introv H S1 S2. split.
-  apply permut_app_l. apply permut_rev.
-  apply~ sorted_app.
-Qed.
-
-Lemma rsorts_app_rev : forall le l1 l2,
- head_le le l2 l1 -> sorted le l1 -> rsorted le l2 ->
- rsorts le (l1 ++ l2) (rev l1 ++ l2).
-Proof using.
-  introv H S1 S2. split.
-  apply permut_app_l. apply permut_rev.
-  apply~ rsorted_app.
-Qed.
-
 Lemma sorts_permut : forall l1 l2 l' le,
-  sorts le l1 l' -> permut l2 l1 ->
+  sorts le l1 l' -> 
+  permut l2 l1 ->
   sorts le l2 l'.
 Proof using.
   introv [P1 S1] Per. split~.
   apply* (@permut_trans _ l1).
 Qed.
 
-Lemma rsorts_permut : forall l1 l2 l' le,
-  rsorts le l1 l' -> permut l2 l1 ->
-  rsorts le l2 l'.
-Proof using. intros. apply~ (@sorts_permut l1). Qed.
-
 Lemma sorts_cons : forall le l l' x,
-  sorts le l l' -> head_of_le le x l' ->
+  sorts le l l' -> 
+  head_le le x l' ->
   sorts le (x::l) (x::l').
 Proof using.
   introv [P S] Hd. split.
-  apply~ permut_cons. apply~ sorted_cons.
+  { apply~ permut_cons. } { apply~ sorted_cons. }
+Qed.
+
+Lemma sorts_length_lt_2 : forall le l,
+  length l < 2 -> 
+  sorts le l l.
+Proof using.
+  intros. apply sorts_refl. destruct~ l.
+  destruct~ l. rew_list in *. false. nat_math.
 Qed.
 
 Lemma sorts_2 : forall le l x1 x2,
@@ -521,20 +467,185 @@ Lemma sorts_2 : forall le l x1 x2,
   sorts le l (x1::x2::nil).
 Proof using.
   intros. apply~ (@sorts_permut (x1::x2::nil)).
-  apply sorts_refl. apply sorted_cons.
-  apply sorted_one. simpls~.
+  apply sorts_refl. apply~ sorted_cons.
 Qed.
 
 Lemma sorts_3 : forall le l x1 x2 x3,
   permut l (x1::x2::x3::nil) ->
-  le x1 x2 -> le x2 x3 ->
+  le x1 x2 -> 
+  le x2 x3 ->
   sorts le l (x1::x2::x3::nil).
 Proof using.
-  intros.
-   apply~ (@sorts_permut (x1::x2::x3::nil)).
-   apply sorts_refl. apply sorted_cons.
-   apply sorted_cons. apply sorted_one.
-   simpls~. simpls~.
+  intros. apply~ (@sorts_permut (x1::x2::x3::nil)).
+  apply sorts_refl. apply~ sorted_cons. 
+  apply~ sorted_cons. 
+Qed.
+
+End Sorts.
+
+
+
+(* ********************************************************************** *)
+(** * Sorting of a list in reverse order *)
+
+(* ---------------------------------------------------------------------- *)
+(** ** [heads_le] *)
+
+(** [heads_le l1 l2] asserts that the head of [l1], if any, is smaller 
+    than the head of [l2], if any. This auxiliary definition is very
+    useful for reasoning about merge-sort style algorithms,
+    especially those involving lists sorted in reverse order (see below). *)
+
+Definition heads_le A (le : binary A) l1 l2 :=
+  match l1,l2 with
+  | _,nil => True
+  | nil,_ => True
+  | h1::_,h2::_ => le h1 h2
+  end.
+
+Section HeadsLe.
+Variables (A : Type).
+Variable le : binary A.
+Hint Resolve sorted_nil sorted_one.
+
+(** Rewriting *)
+
+Lemma heads_le_cons_l : forall x l1 l2,
+  heads_le le (x::l1) l2 = head_le le x l2.
+Proof using. intros. destruct~ l2. Qed.
+
+Lemma heads_le_cons_r : forall x l1 l2,
+  heads_le le l1 (x::l2) = head_le le x l1.
+Proof using. intros. destruct~ l1. Qed.
+
+Lemma heads_le_nil_l : forall l,
+  heads_le le nil l.
+Proof using. intros. unfolds. destruct~ l. Qed.
+
+Lemma heads_le_nil_r : forall l,
+  heads_le le l nil.
+Proof using. intros. unfolds. destruct~ l. Qed.
+
+(** Simplification for flip *)
+
+Lemma heads_le_flip_eq : forall l1 l2,
+  heads_le (flip le) l1 l2 = heads_le le l2 l1.
+Proof using. destruct l1; destruct l2; auto. Qed.
+
+Lemma heads_le_flip : forall l1 l2,
+  heads_le le l2 l1 -> 
+  heads_le (flip le) l1 l2.
+Proof using. intros. rewrite~ heads_le_flip_eq. Qed.
+
+Lemma heads_le_flip_inv : forall l1 l2,
+  heads_le (flip le) l1 l2 -> 
+  heads_le le l2 l1.
+Proof using. intros. rewrite~ <- heads_le_flip_eq. Qed.
+
+End HeadsLe.
+
+
+(* ---------------------------------------------------------------------- *)
+(** ** [rsorted] *)
+
+(** [rsorted le l] asserts that [l] is sorted in reverse order 
+    w.r.t. [le]. *)
+
+Definition rsorted A (le : binary A) := sorted (flip le).
+
+Section RSorted.
+Variables (A : Type) (le : binary A).
+Implicit Types l : list A.
+Hint Constructors sorted.
+Hint Resolve sorted_nil sorted_one.
+Hint Unfold rsorted.
+
+(** Constructors *)
+
+Lemma rsorted_nil : rsorted le nil.
+Proof using. applys sorted_nil. Qed.
+
+Lemma rsorted_one : forall x,
+  rsorted le (x::nil).
+Proof using. intros. applys sorted_one. Qed.
+
+Lemma rsorted_two : forall x y l,
+  rsorted le (y::l) -> 
+  le y x ->
+  rsorted le (x::y::l).
+Proof using. intros. applys* sorted_two. Qed.
+
+Lemma rsorted_cons : forall l x,
+  rsorted le l ->
+  head_le (flip le) x l ->
+  rsorted le (x::l).
+Proof using. introv S H. inverts~ S. Qed.
+
+(** Inversion *)
+
+Lemma rsorted_cons_inv : forall x l,
+  rsorted le (x::l) -> 
+  head_le (flip le) x l /\ rsorted le l.
+Proof using. introv H. inverts H; simpls~. Qed.
+
+Lemma rsorted_cons_inv_head_le : forall x l1 l2,
+  rsorted le (x::l2) ->
+  head_le (flip le) x l2.
+Proof using. introv E. forwards*: rsorted_cons_inv E. Qed.
+
+End RSorted.
+
+(** Append of a the reverse of a [rsorted] list and a [sorted] list. *)
+
+Lemma sorted_app_rev : forall (A : Type) (le : binary A) l1 l2,
+  heads_le le l1 l2 -> 
+  rsorted le l1 -> 
+  sorted le l2 ->
+  sorted le ((rev l1) ++ l2).
+Proof using.
+  introv. gen l2. induction l1; introv Hd S1 S2; rew_list.
+  { auto. }
+  { rewrite heads_le_cons_l in Hd.
+    lets (Hd1&S1'): rsorted_cons_inv (rm S1).
+    apply~ IHl1. apply~ sorted_cons. }
+Qed.
+
+(** Append of a the reverse of a [sorted] list and a [rsorted] list. *)
+
+Lemma rsorted_app_rev : forall (A : Type) (le : binary A) l1 l2,
+  heads_le le l2 l1 -> 
+  sorted le l1 -> 
+  rsorted le l2 ->
+  rsorted le ((rev l1) ++ l2).
+Proof using.
+  unfold rsorted. intros. apply~ sorted_app_rev.
+  rewrite~ heads_le_flip_eq.
+Qed.
+
+
+(* ---------------------------------------------------------------------- *)
+(** ** [rsorts] *)
+
+(** [rsorts le l l'] asserts that [l'] is the result of sorting
+    [l] in reverse order w.r.t. [le]. *)
+
+Definition rsorts A (le : binary A) := sorts (flip le).
+
+Section Rsorts.
+Variables (A : Type).
+Implicit Types le : binary A.
+Hint Resolve sorted_nil sorted_one.
+
+Lemma rsorts_refl : forall le l,
+  rsorted le l -> 
+  rsorts le l l.
+Proof using. intros. apply~ sorts_refl. Qed.
+
+Lemma sorts_cons : forall le l l' x,
+  rsorts le l l' -> 
+  head_le (flip le) x l' ->
+  rsorts le (x::l) (x::l').
+Proof using.
 Qed.
 
 Lemma rsorts_2 : forall le l x1 x2,
@@ -550,7 +661,8 @@ Qed.
 
 Lemma rsorts_3 : forall le l x1 x2 x3,
   permut l (x1::x2::x3::nil) ->
-  le x2 x1 -> le x3 x2 ->
+  le x2 x1 -> 
+  le x3 x2 ->
   rsorts le l (x1::x2::x3::nil).
 Proof using.
   intros.
@@ -560,14 +672,24 @@ Proof using.
    simpls~. simpls~.
 Qed.
 
-Lemma sorts_length_lt_2 : forall le l,
-  length l < 2 -> sorts le l l.
+Lemma rsorts_permut : forall l1 l2 l' le,
+  rsorts le l1 l' -> 
+  permut l2 l1 ->
+  rsorts le l2 l'.
+Proof using. intros. apply~ (@sorts_permut l1). Qed.
+
+
+(* LATER
+Lemma rsorts_app_rev : forall le l1 l2,
+ heads_le le l2 l1 -> 
+ sorted le l1 -> 
+ rsorted le l2 ->
+ rsorts le (l1 ++ l2) (rev l1 ++ l2).
 Proof using.
-  intros. apply sorts_refl. destruct~ l.
-  destruct~ l. rew_length in *. false. nat_math.
+  introv H S1 S2. split.
+  apply permut_app_l. apply permut_rev.
+  apply~ rsorted_app.
 Qed.
+*)
 
-End Sorts.
-
-
-
+End Rsorts.
