src/LibSet.v
@@ -1017,7 +1017,7 @@ Proof using.
   apply~ foreach_single.
 Qed.
 
-Lemma foreach_weaken : forall P Q E,
+Lemma foreach_pred_ld: forall P Q E,
   foreach P E -> pred_le P Q -> foreach Q E.
 Proof using. introv H L K. apply~ L. Qed.
 
